PeanoRF.lean
@@ -14,11 +14,12 @@ import PeanoRF.Calculus.Consistency
 import PeanoRF.Calculus.DerivesI
 import PeanoRF.Calculus.Eq
 import PeanoRF.Calculus.Slash
+import PeanoRF.Calculus.Soundness
 import PeanoRF.Calculus.Subst
 import PeanoRF.Calculus.SubstDerives
-import PeanoRF.Calculus.Soundness
 import PeanoRF.HA.Arith
 import PeanoRF.HA.Axioms
+import PeanoRF.HA.Domain
 import PeanoRF.HA.Numerals
 import PeanoRF.Meta.AxiomCheck
 import PeanoRF.Omega.Basic
